theories/cast_calculus/consistency/structural.v
@@ -1,4 +1,5 @@
 From Autosubst Require Export Autosubst.
+From fae_gtlc_mu.stlc_mu Require Export typing.
 From fae_gtlc_mu.cast_calculus Require Export types.
 From fae_gtlc_mu Require Import prelude.
 Require Coq.Logic.JMeq.
@@ -8,63 +9,110 @@ Inductive Assumption : Type :=
   | LogBodies (τ1 τ2 : type) (P1 : not (τ1 = ⋆)) (P2 : ¬ (τ2 = ⋆)) : Assumption
   | LogStar : Assumption. (* can be of μ.τ ~ μ.⋆ or μ.⋆ ~ μ.τ *)
 
-(*
-Inductive Shape : Type :=
-  | Arrow
-  | Sum
-  | Prod
-  | Rec.
-*)
+(** ######################################################################## *)
 
-
-(* possibly with sigma type and proof of groundness *)
-Definition get_shape (τ : type) : option type :=
-  match τ with
-  | TUnit => None
-  | TProd x x0 => Some (TProd ⋆ ⋆)
-  | TSum x x0 => Some (TSum ⋆ ⋆)
-  | TArrow x x0 => Some (TArrow ⋆ ⋆)
-  | TRec τ => Some (TRec ⋆)
-  | TVar x => Some (TRec ⋆)
-  | TUnknown => None
+Definition helper1 (a : Assumption) : (type * type) :=
+  match a with
+  | Unfolded => (TUnit , TUnit)
+  | LogBodies τ1 τ2 P1 P2 => (TRec τ1 , TRec τ2)
+  | LogStar => (TUnit , TUnit)
   end.
 
-(*
-Definition to_ground (τ : type) : option type :=
-  match τ with
-  | TUnit => None
-  | TProd τ1 τ2 => match (Is_Unknown_dec τ1) with
-                    | left _ => match (Is_Unknown_dec τ2) with
-                               | left _ => None
-                               | right _ => Some (⋆ × ⋆)
-                             end
-                    | right _ => Some (⋆ × ⋆)
-                  end
-  | TSum τ1 τ2 => match (Is_Unknown_dec τ1) with
-                    | left _ => match (Is_Unknown_dec τ2) with
-                               | left _ => None
-                               | right _ => Some (⋆ + ⋆)%type
-                             end
-                    | right _ => Some (⋆ + ⋆)%type
-                  end
-  | TArrow τ1 τ2 => match (Is_Unknown_dec τ1) with
-                    | left _ => match (Is_Unknown_dec τ2) with
-                               | left _ => None
-                               | right _ => Some (TArrow ⋆ ⋆)%type
-                             end
-                    | right _ => Some (TArrow ⋆ ⋆)%type
-                  end
-  | TRec τ => match (Is_Unknown_dec τ) with
-               | left _ => None
-               | right _ => Some (TRec ⋆)
-             end
-  | TVar x => Some (TRec ⋆)
-  | TUnknown => None
+Fixpoint close_up (τ1τ2 : type * type) (Γ : list (type * type)) :=
+  match Γ with
+  | nil => τ1τ2
+  | cons τ1'τ2' Γ' => close_up ((fst τ1τ2).[fst τ1τ2/] , (snd τ1τ2).[snd τ1τ2/]) Γ'
   end.
+
+Fixpoint close_up_list (Γ : list (type * type)) : list (type * type) :=
+  match Γ with
+  | nil => nil
+  | cons openτ openΓ => (close_up openτ openΓ) :: (close_up_list openΓ)
+  end.
+
+Definition assumptions_to_closed_gradual_pairs (A : list Assumption) : list (type * type) :=
+  close_up_list (fmap helper1 A).
+
+(*
+Fixpoint subs_list (τ : type) (Γ : list type) :=
+  match Γ with
+  | nil => τ
+  | cons τ' Γ' => subs_list τ.[τ'/] Γ'
+  end.
+
+Fixpoint close_up (openΓ : list type) : list type :=
+  match openΓ with
+  | nil => nil
+  | cons openτ openΓ => subs_list openτ openΓ :: (close_up openΓ)
+  end.
+
+Definition assumptions_to_initial_gradual_context (A : list Assumption) : list type :=
+  close_up (map (compose fst assumption_to_open_pair) A).
+
+Definition assumptions_to_final_gradual_context (A : list Assumption) : list type :=
+  close_up (map (compose snd assumption_to_open_pair) A).
+
+Definition assumptions_to_gradual_pairs (A : list Assumption) : list (type * type) :=
+  zip (assumptions_to_initial_gradual_context A)
+      (assumptions_to_final_gradual_context A).
 *)
 
-Definition update {A : Type} (l : list A) (i : nat) (a : A) : list A :=
-  alter (fun _ => a) i l.
+(** ######################################################################## *)
+
+
+Inductive UBAssumptions : list Assumption -> Type :=
+  | empty : UBAssumptions []
+  | consUnfolded A : UBAssumptions A -> UBAssumptions (Unfolded :: A)
+  | consLogStar A : UBAssumptions A -> UBAssumptions (LogStar :: A)
+  | consLogBodies A τ1 τ2 P1 P2 :
+      UBAssumptions A -> UB (S (length A)) τ1 -> UB (S (length A)) τ2 -> UBAssumptions (LogBodies τ1 τ2 P1 P2 :: A).
+          (* we only need n = 0? *)
+
+Lemma ubass1 A x : UBAssumptions A -> UBAssumptions (update A x Unfolded).
+Admitted.
+
+Definition UBAssumption (a : Assumption) (n : nat) : Type :=
+  match a with
+  | Unfolded => True
+  | LogBodies τ1 τ2 P1 P2 => UB n τ1 * UB n τ2
+  | LogStar => True
+  end.
+
+Lemma ubass2 A (PAub : UBAssumptions A) x τ1 τ2 P1 P2 (eq : A !! x = Some (LogBodies τ1 τ2 P1 P2)) : UB (length A) τ1.
+Admitted.
+
+Definition flip (A : Assumption) : Assumption :=
+  match A with
+  | Unfolded => Unfolded
+  | LogBodies τ1 τ2 P1 P2 => LogBodies τ2 τ1 P2 P1
+  | LogStar => LogStar
+  end.
+
+Lemma ubass_flip A : UBAssumptions A -> UBAssumptions (map flip A).
+Admitted.
+
+Lemma flipflip a : flip (flip a) = a.
+  by destruct a.
+Qed.
+
+Lemma flipflipmap l : map flip (map flip l) = l.
+  induction l.
+  by simpl.
+  simpl. by rewrite flipflip IHl.
+Qed.
+
+Lemma map_lookup (l : list Assumption) (f : Assumption -> Assumption) (i : nat) (a : Assumption) :
+  l !! i = Some (f a) -> ((map f l) !! i = Some a).
+Proof.
+Admitted.
+
+Lemma map_update (f : Assumption -> Assumption) (l : list Assumption) i a :
+  map f (update l i a) = update (map f l) i (f a).
+Proof.
+Admitted.
+
+
+
 
 Reserved Notation "A ⊢ τ ~ τ'" (at level 4, τ, τ' at next level).
 Inductive cons_struct (A : list Assumption) : type -> type -> Type :=
@@ -135,9 +183,9 @@ Inductive cons_struct (A : list Assumption) : type -> type -> Type :=
   (** Variables *)
   (* consuming assumption; using previously exposed recursive call *)
   (* | consUseRecursion i : *)
-  | consUseRecursion i τb τb' P P' :
-      (A !! i) = Some (LogBodies τb τb' P P') -> (* we will only need rule with = Some (LogBodies ... )*)
-      (* i < length A -> *)
+  | consUseRecursion i :
+      (* (A !! i) = Some a -> (* we will only need rule with = Some (LogBodies ... )*) *)
+      i < length A ->
       (* is_Some (A !! i) -> *)
       A ⊢ (TVar i) ~ (TVar i)
   | consUseRecursionLStar i :
@@ -165,3 +213,5 @@ Inductive cons_struct (A : list Assumption) : type -> type -> Type :=
       (* A ⊢ (TRec ⋆) ~ (TVar i) -> *)
       (* A ⊢ ⋆ ~ (TVar i) *)
 where "A ⊢ τ ~ τ'" := (cons_struct A τ τ').
+
+
