theories/prelude.v
@@ -5,3 +5,19 @@ From iris.algebra Require Export base.
 Definition TDecision : Type -> Type := λ P : Type, sum P (P -> False).
 
 (* Definition TNeg : Type -> Type := λ P : Type, P → False. *)
+
+From Autosubst Require Export Autosubst.
+
+Section Autosubst_Lemmas.
+  Context {term : Type} {Ids_term : Ids term}
+          {Rename_term : Rename term} {Subst_term : Subst term}
+          {SubstLemmas_term : SubstLemmas term}.
+
+  Lemma iter_up (m x : nat) (f : var → term) :
+    upn m f x = if lt_dec x m then ids x else rename (+m) (f (x - m)).
+  Proof.
+    revert x; induction m as [|m IH]=> -[|x];
+      repeat (destruct (lt_dec _ _) || asimpl || rewrite IH); auto with lia.
+  Qed.
+End Autosubst_Lemmas.
+
