theories/stlc_mu/lib/cast_emulations/between.v
@@ -1,0 +1,88 @@
+From fae_gtlc_mu.cast_calculus Require Export types consistency.structural.
+From fae_gtlc_mu.stlc_mu Require Export typing lang lib.fix.
+From fae_gtlc_mu.stlc_mu.lib Require Export universe.
+From fae_gtlc_mu.backtranslation Require Export types.
+
+(** Between sums, products, recursive types, arrow types *)
+
+Definition between_TSum (c1 c2 : expr) : expr :=
+  Lam (Case (Var 0) (InjL ((rename (+2) c1) (Var 0))) (InjR ((rename (+2) c2) (Var 0)))).
+
+Lemma between_TSum_typed Γ (τ1 τ2 τ1' τ2' : cast_calculus.types.type) (f1 f2 : expr) (d1 : Γ ⊢ₛ f1 : (<<τ1>> → <<τ1'>>)) (d2 : Γ ⊢ₛ f2 : (<<τ2>> → <<τ2'>>)) :
+  Γ ⊢ₛ between_TSum f1 f2 : (<<τ1>> + <<τ2>> → <<τ1'>> + <<τ2'>>)%type.
+Proof.
+  apply Lam_typed.
+  apply Case_typed with (τ1 := <<τ1>>) (τ2 := <<τ2>>).
+  by apply Var_typed.
+  constructor. eapply App_typed.
+  apply up_type_two. apply d1.
+  by apply Var_typed.
+  constructor. eapply App_typed.
+  apply up_type_two. apply d2. by apply Var_typed.
+Qed.
+
+Definition between_TProd (f1 f2 : expr) : expr :=
+  Lam (Pair (rename (+1) f1 (Fst (Var 0))) (rename (+1) f2 (Snd (Var 0)))).
+
+Lemma between_TProd_typed Γ (τ1 τ2 τ1' τ2' : cast_calculus.types.type) (f1 f2 : expr) (d1 : Γ ⊢ₛ f1 : (<<τ1>> → <<τ1'>>)) (d2 : Γ ⊢ₛ f2 : (<<τ2>> → <<τ2'>>)) :
+  Γ ⊢ₛ between_TProd f1 f2 : ((<<τ1>> × <<τ2>>) → (<<τ1'>> × <<τ2'>>))%type.
+Proof.
+  apply Lam_typed.
+  apply Pair_typed.
+  eapply App_typed.
+  apply up_type_one. apply d1. econstructor. by apply Var_typed.
+  eapply App_typed.
+  apply up_type_one. apply d2. econstructor. by apply Var_typed.
+Qed.
+
+Definition between_TArrow (ca cr : expr) : expr :=
+  Lam (*f*)
+    (Lam (*a*) (
+         rename (+2) cr (((Var 1)(*f*)) (rename (+2) ca (Var 0(*a*))))
+       )
+    ).
+
+Lemma between_TArrow_typed Γ (τ1 τ2 τ3 τ4 : cast_calculus.types.type) (ca cr : expr) (da : Γ ⊢ₛ ca : (<<τ3>> → <<τ1>>)) (dr : Γ ⊢ₛ cr : (<<τ2>> → <<τ4>>)) :
+  Γ ⊢ₛ between_TArrow ca cr : ((<<τ1>> → <<τ2>>) → (<<τ3>> → <<τ4>>))%type.
+Proof.
+  repeat apply Lam_typed.
+  apply App_typed with (τ1 := <<τ2>>).
+  auto. apply up_type_two. apply dr. apply App_typed with (τ1 := <<τ1>>).
+    by auto; apply Var_typed.
+    eapply App_typed. by apply up_type_two.
+    by apply Var_typed.
+Qed.
+
+Definition between_TRec (f : expr) : expr :=
+  Lam (* x : μ. <<τi.[...]>> *) (
+      Fix (
+          Lam (* g : μ.<<τi.[...]>> → μ.<<τf.[...]>> *) (
+              Lam (* r : μ.<<τi.[...]>> *) (
+                  Fold (rename (+3) f(*<<τi.[μ.τi/]>>*) (Unfold (Var 0)))
+                )
+            )
+        ) (Var 0)
+    ).
+
+From fae_gtlc_mu.cast_calculus Require Import types. (* make use of subs notation in gtlc *)
+
+Lemma between_TRec_typed Γ (τi τf : cast_calculus.types.type) (Pi : Is_Closed (TRec τi)) (Pf : Is_Closed (TRec τf)) (f : expr)
+      (d : Γ ⊢ₛ f : (<<(τi.[TRec τi/])>> → <<τf.[TRec τf/]>>)) :
+  Γ ⊢ₛ between_TRec f : ((stlc_mu.typing.TRec <<τi>>) → (stlc_mu.typing.TRec <<τf>>))%type.
+From fae_gtlc_mu.stlc_mu Require Export typing.
+Proof.
+  apply Lam_typed.
+  apply App_typed with (τ1 := TRec <<τi>>).
+  apply App_typed with (τ1 := ((TRec << τi >> → TRec << τf >>) → (TRec << τi >> → TRec << τf >>))).
+  apply Fix_typed.
+  admit.
+  apply Lam_typed.
+  apply Lam_typed.
+  apply Fold_typed.
+  apply App_typed with (τ1 := <<τi>>.[(TRec <<τi>>)/]).
+  apply up_type_three.
+  admit.
+  apply Unfold_typed.
+    by apply Var_typed.
+    by apply Var_typed.
+Admitted.
