theories/stlc_mu/lib/cast_emulations/embed.v
@@ -1,0 +1,84 @@
+From fae_gtlc_mu.cast_calculus Require Export types consistency.structural.
+From fae_gtlc_mu.stlc_mu Require Export typing lang lib.fix lib.universe.
+From fae_gtlc_mu.backtranslation Require Export types.
+
+(** Embeddings *)
+
+Definition embed_TUnit : expr :=
+  Lam (Fold (InjL (InjL (InjL (InjL (Var 0)))))).
+
+Lemma embed_TUnit_typed Γ :
+  Γ ⊢ₛ embed_TUnit : (TUnit → Universe).
+Proof.
+  apply Lam_typed, Fold_typed.
+  repeat apply InjL_typed.
+  by apply Var_typed.
+Qed.
+
+Definition embed_Ground_TSum : expr :=
+  Lam (Fold ((InjL (InjL (InjL (InjR (Var 0))))))).
+
+Definition embed_Ground_TSum_typed Γ :
+  Γ ⊢ₛ embed_Ground_TSum : ((Universe + Universe) → Universe)%type.
+Proof.
+  apply Lam_typed.
+  apply Fold_typed.
+  repeat apply InjL_typed. apply InjR_typed.
+  by apply Var_typed.
+Qed.
+
+Definition embed_Ground_TProd : expr :=
+  Lam (Fold (InjL (InjL (InjR (Var 0))))).
+
+Definition embed_Ground_TProd_typed Γ :
+  Γ ⊢ₛ embed_Ground_TProd : ((Universe × Universe) → Universe).
+Proof.
+  apply Lam_typed, Fold_typed.
+  repeat apply InjL_typed. asimpl. repeat apply InjR_typed.
+  by apply Var_typed.
+Qed.
+
+Definition embed_Ground_TArrow : expr :=
+  Lam (Fold (InjL (InjR (Var 0)))).
+
+Definition embed_Ground_TArrow_typed Γ :
+  Γ ⊢ₛ embed_Ground_TArrow : ((Universe → Universe) → Universe).
+Proof.
+  apply Lam_typed, Fold_typed.
+  repeat apply InjL_typed. asimpl. repeat apply InjR_typed.
+  by apply Var_typed.
+Qed.
+
+(* Takes something of μ.Universe, unfolds it so it is in Universe, and then puts in the last branch of the universe *)
+Definition embed_Ground_TRec : expr :=
+  Lam (Fold (InjR (Unfold (Var 0)))).
+
+Definition embed_Ground_TRec_typed Γ :
+  Γ ⊢ₛ embed_Ground_TRec : (TRec Universe → Universe).
+Proof.
+  apply Lam_typed. apply Fold_typed.
+  apply InjR_typed.
+  asimpl.
+  apply Unfold_typed_help; first by trivial.
+  by apply Var_typed.
+Qed.
+
+Definition embed (τ : cast_calculus.types.type) (G : Ground τ) : expr :=
+  match G with
+  | Ground_TUnit => embed_TUnit
+  | Ground_TProd => embed_Ground_TProd
+  | Ground_TSum => embed_Ground_TSum
+  | Ground_TArrow => embed_Ground_TArrow
+  | Ground_TRec => embed_Ground_TRec
+  end.
+
+Lemma embed_typed {τG : cast_calculus.types.type} {G : Ground τG} Γ :
+  Γ ⊢ₛ (embed τG G) : (<<τG>> → Universe).
+Proof.
+  destruct G.
+    + apply embed_TUnit_typed.
+    + apply embed_Ground_TProd_typed.
+    + apply embed_Ground_TSum_typed.
+    + apply embed_Ground_TArrow_typed.
+    + apply embed_Ground_TRec_typed.
+Qed.
