theories/stlc_mu/lib/cast_emulations/extract.v
@@ -1,0 +1,181 @@
+From fae_gtlc_mu.cast_calculus Require Export types consistency.structural.
+From fae_gtlc_mu.stlc_mu Require Export typing lang lib.fix lib.universe.
+From fae_gtlc_mu.backtranslation Require Export types.
+
+(** Extractions *)
+
+Definition Ω : expr :=
+  (
+    (Lam ((Unfold (Var 0)) (Var 0)))
+      (Fold (Lam ((Unfold (Var 0)) (Var 0))))
+  ).
+
+Definition Ω_typed Γ τ : (Is_Closed τ) -> (Γ ⊢ₛ Ω : τ).
+Proof.
+  intro P.
+  apply App_typed with (τ1 := (TRec (TVar 0 → τ))).
+  - apply Lam_typed.
+    apply App_typed with (τ1 := TRec (TVar 0 → τ)).
+    + apply Unfold_typed_help_2 with (τ := (TVar 0 → τ)).
+      asimpl. by rewrite P. by apply Var_typed.
+    + by apply Var_typed.
+  - apply Fold_typed. asimpl. rewrite P.
+    apply Lam_typed.
+    apply App_typed with (τ1 := TRec (TVar 0 → τ)).
+    + apply Unfold_typed_help_2 with (τ := (TVar 0 → τ)).
+      asimpl. by rewrite P. by apply Var_typed.
+    + by apply Var_typed.
+Qed.
+
+Definition extract_TUnit : expr :=
+  Lam (Case (Unfold (Var 0))
+            (Case (Var 0)
+                  (Case (Var 0)
+                        (Case (Var 0)
+                              (Var 0)
+                              (Ω)
+                        )
+                        (Ω)
+                  )
+                  (Ω)
+            )
+            (Ω)
+      ).
+
+Definition extract_TUnit_typed Γ : Γ ⊢ₛ extract_TUnit : (Universe → TUnit).
+Proof.
+  apply Lam_typed.
+  apply Case_typed with (τ1 := (TUnit + (TVar 0 + TVar 0) + (TVar 0 × TVar 0) + (TVar 0 → TVar 0)).[Universe/]%type)
+                         (τ2 := Universe).
+  - eapply Unfold_typed_help_2 with (τ := Universe_body). by asimpl.
+    by apply Var_typed.
+  - apply Case_typed with (τ1 := (TUnit + (TVar 0 + TVar 0) + (TVar 0 × TVar 0)).[Universe/]%type)
+                          (τ2 := (TVar 0 → TVar 0).[Universe/]%type).
+    + by apply Var_typed.
+    + eapply Case_typed.
+      * by apply Var_typed.
+      * eapply Case_typed.
+        -- by apply Var_typed.
+        -- by apply Var_typed.
+        -- by apply Ω_typed.
+      * by apply Ω_typed.
+    + by apply Ω_typed.
+  - by apply Ω_typed.
+Qed.
+
+Definition extract_Ground_TSum : expr :=
+  Lam (Case (Unfold (Var 0))
+            (Case (Var 0)
+                  (Case (Var 0)
+                        (Case (Var 0)
+                              (Ω)
+                              (Var 0)
+                        )
+                        (Ω)
+                  )
+                  (Ω)
+            )
+            (Ω)
+      ).
+
+Definition extract_Ground_TSum_typed Γ : Γ ⊢ₛ extract_Ground_TSum : (Universe → (Universe + Universe))%type.
+Proof.
+  apply Lam_typed.
+  apply Case_typed with (τ1 := (TUnit + (TVar 0 + TVar 0) + (TVar 0 × TVar 0) + (TVar 0 → TVar 0)).[Universe/]%type)
+                         (τ2 := Universe).
+  - eapply Unfold_typed_help_2 with (τ := Universe_body). by asimpl. by apply Var_typed.
+  - eapply Case_typed. by apply Var_typed.
+    + eapply Case_typed.
+      * by apply Var_typed.
+      * eapply Case_typed.
+        -- by apply Var_typed.
+        -- by apply Ω_typed.
+        -- by apply Var_typed.
+      * by apply Ω_typed.
+    + by apply Ω_typed.
+  - by apply Ω_typed.
+Qed.
+
+Definition extract_Ground_TProd : expr :=
+  Lam (Case (Unfold (Var 0))
+            (Case (Var 0)
+                  (Case (Var 0)
+                        (Ω)
+                        (Var 0)
+                  )
+                  (Ω)
+            )
+            (Ω)
+      ).
+
+Definition extract_Ground_TProd_typed Γ : Γ ⊢ₛ extract_Ground_TProd : (Universe → (Universe × Universe)).
+Proof.
+  apply Lam_typed.
+  apply Case_typed with (τ1 := (TUnit + (TVar 0 + TVar 0) + (TVar 0 × TVar 0) + (TVar 0 → TVar 0)).[Universe/]%type)
+                         (τ2 := Universe).
+  - eapply Unfold_typed_help_2 with (τ := Universe_body). by asimpl. by apply Var_typed.
+  - eapply Case_typed. by apply Var_typed.
+    + eapply Case_typed.
+      * by apply Var_typed.
+      * by apply Ω_typed.
+      * by apply Var_typed.
+    + by apply Ω_typed.
+  - by apply Ω_typed.
+Qed.
+
+Definition extract_Ground_TArrow : expr :=
+  Lam (Case (Unfold (Var 0))
+            (Case (Var 0)
+                  (Ω)
+                  (Var 0)
+            )
+            (Ω)
+      ).
+
+Definition extract_Ground_TArrow_typed Γ : Γ ⊢ₛ extract_Ground_TArrow : (Universe → (Universe → Universe)).
+Proof.
+  apply Lam_typed.
+  apply Case_typed with (τ1 := (TUnit + (TVar 0 + TVar 0) + (TVar 0 × TVar 0) + (TVar 0 → TVar 0)).[Universe/]%type)
+                         (τ2 := Universe).
+  - eapply Unfold_typed_help_2 with (τ := Universe_body). by asimpl. by apply Var_typed.
+  - eapply Case_typed. by apply Var_typed.
+    + by apply Ω_typed.
+    + by apply Var_typed.
+  - by apply Ω_typed.
+Qed.
+
+Definition extract_Ground_TRec : expr :=
+  Lam (Case (Unfold (Var 0))
+            (Ω)
+            (Fold (Var 0))
+      ).
+
+Definition extract_Ground_TRec_typed Γ : Γ ⊢ₛ extract_Ground_TRec : (Universe → TRec Universe).
+Proof.
+  apply Lam_typed.
+  apply Case_typed with (τ1 := (TUnit + (TVar 0 + TVar 0) + (TVar 0 × TVar 0) + (TVar 0 → TVar 0)).[Universe/]%type)
+                         (τ2 := Universe).
+  - eapply Unfold_typed_help_2 with (τ := Universe_body). by asimpl. by apply Var_typed.
+  - by apply Ω_typed.
+  - apply Fold_typed. by apply Var_typed.
+Qed.
+
+Definition extract (τ : cast_calculus.types.type) (G : Ground τ) : expr :=
+  match G with
+  | Ground_TUnit => extract_TUnit
+  | Ground_TProd => extract_Ground_TProd
+  | Ground_TSum => extract_Ground_TSum
+  | Ground_TArrow => extract_Ground_TArrow
+  | Ground_TRec => extract_Ground_TRec
+  end.
+
+Lemma extract_typed {τG : cast_calculus.types.type} {G : Ground τG} Γ :
+  Γ ⊢ₛ (extract τG G) : (Universe → <<τG>>).
+Proof.
+  destruct G.
+    + apply extract_TUnit_typed.
+    + apply extract_Ground_TProd_typed.
+    + apply extract_Ground_TSum_typed.
+    + apply extract_Ground_TArrow_typed.
+    + apply extract_Ground_TRec_typed.
+Qed.
