theories/stlc_mu/lib/cast_emulations/factorize.v
@@ -1,0 +1,49 @@
+From fae_gtlc_mu.cast_calculus Require Export types consistency.structural.
+From fae_gtlc_mu.stlc_mu Require Export typing lang lib.fix.
+From fae_gtlc_mu.stlc_mu.lib Require Export universe embed extract.
+From fae_gtlc_mu.backtranslation Require Export types.
+
+(** Trivial stuff *)
+
+Definition identity : expr :=
+  Lam (Var 0).
+
+Lemma identity_typed (τ : type) Γ : Γ ⊢ₛ identity : (τ → τ).
+Proof.
+  intros.
+  apply Lam_typed. by apply Var_typed.
+Qed.
+
+(** Factorisations *)
+
+Definition factorization_up (f : expr) (τG : cast_calculus.types.type) (G : Ground τG) : expr :=
+  Lam (
+      embed τG G ((rename (+1) f) (Var 0))
+    ).
+
+Lemma factorization_up_typed Γ {f : expr} (τ τG : cast_calculus.types.type) (G : Ground τG) (p1 : (Ground τ -> False)) (p2 : not (τ = ⋆)) (d : Γ ⊢ₛ f : (<<τ>> → <<τG>>)) :
+  Γ ⊢ₛ factorization_up f τG G : (<<τ>> → Universe).
+Proof.
+  apply Lam_typed.
+  apply App_typed with (τ1 := << τG >>).
+  apply embed_typed.
+  apply App_typed with (τ1 := << τ >>).
+  apply up_type_one. apply d.
+  by apply Var_typed.
+Qed.
+
+Definition factorization_down (f : expr) (τG : cast_calculus.types.type) (G : Ground τG) : expr :=
+  Lam (
+      (rename (+1) f) (extract τG G (Var 0))
+    ).
+
+Lemma factorization_down_typed Γ {f : expr} (τ τG : cast_calculus.types.type) (G : Ground τG) (p1 : notT (Ground τ)) (p2 : not (τ = ⋆)) (d : Γ ⊢ₛ f : (<<τG>> → <<τ>>)) :
+  Γ ⊢ₛ factorization_down f τG G : (Universe → <<τ>>).
+Proof.
+  apply Lam_typed.
+  apply App_typed with (τ1 := << τG >>).
+  apply up_type_one. apply d.
+  apply App_typed with (τ1 := Universe).
+  apply extract_typed.
+  by apply Var_typed.
+Qed.
