theories/stlc_mu/lib/cast_emulations/general.v
@@ -1,0 +1,133 @@
+From fae_gtlc_mu.cast_calculus Require Export types consistency.structural.
+From fae_gtlc_mu.stlc_mu Require Export typing lang lib.fix.
+From fae_gtlc_mu.stlc_mu.lib Require Export universe.
+From fae_gtlc_mu.stlc_mu.lib.cast_emulations Require Export embed factorize extract between.
+From fae_gtlc_mu.backtranslation Require Export types.
+
+(** emulation of a cast between an arbitrary pair of consistent types *)
+(* recursively defined on the alternative consistency relation *)
+
+Fixpoint 𝓕 (A : list Assumption) (τi τf : cast_calculus.types.type) (P : A ⊢ τi ~ τf) : expr :=
+  match P with
+  | consStarTGround _ τ G (* ⋆ ~ G *) => extract τ G
+  | consTGroundStar _ τ G (* G ~ ⋆ *) => embed τ G
+  | consTauStar _ τ τG pUB nGτ nSτ pshapeτ PττG =>
+    factorization_up (𝓕 A τ τG PττG) τG (get_shape_is_ground pshapeτ)
+  | consStarTau _ τ τG pUB nGτ nSτ pshapeτ PττG =>
+    factorization_down (𝓕 A τG τ PττG) τG (get_shape_is_ground pshapeτ)
+  | consBaseBase _ => identity
+  | consStarStar _ => identity
+  | consTSumTSum _ τ1 τ1' τ2 τ2' P1 P2 =>
+    between_TSum
+      (𝓕 A τ1 τ1' P1)
+      (𝓕 A τ2 τ2' P2)
+  | consTProdTProd _ τ1 τ1' τ2 τ2' P1 P2 =>
+    between_TProd
+      (𝓕 A τ1 τ1' P1)
+      (𝓕 A τ2 τ2' P2)
+  | consTArrowTArrow _ τ1 τ2 τ3 τ4 P31 P24 =>
+    between_TArrow
+      (𝓕 A τ3 τ1 P31)
+      (𝓕 A τ2 τ4 P24)
+  | consExposeRecursion _ τi τf PτinS PτfnS Pτiτf =>
+    between_TRec (𝓕 (LogBodies τi τf PτinS PτfnS :: _) τi τf Pτiτf)
+  | consExposeRecursionLStar _ τ P => Unit
+  | consExposeRecursionRStar _ τ P => Unit
+  | consExposeExtraRecursionRStar _ i τb τb' P P' x x0 => Unit
+  | consExposeExtraRecursionLStar _ i τb τb' P P' x x0 => Unit
+  | consUseRecursion _ i x => Var i
+  | consUseRecursionLStar _ i x => Var i
+  | consUseRecursionRStar _ i x => Var i
+  | consUseExtraRecursionLStar _ i x => Var i
+  | consUseExtraRecursionRStar _ i x => Var i
+  end.
+
+Definition closed_gradual_pair_to_type (ττ' : cast_calculus.types.type * cast_calculus.types.type) : type :=
+  match ττ' with
+  | pair τ τ' => TArrow (backtranslate_type τ) (backtranslate_type τ')
+  end.
+
+Definition assumptions_to_context (A : list Assumption) : list type :=
+  map closed_gradual_pair_to_type (assumptions_to_closed_gradual_pairs A).
+
+Definition initial_type (τi τf : cast_calculus.types.type) (A : list Assumption) : type :=
+  backtranslate_type $ fst (close_up (τi, τf) (assumptions_to_closed_gradual_pairs A)).
+
+Definition final_type (τi τf : cast_calculus.types.type) (A : list Assumption) : type :=
+  backtranslate_type $ snd (close_up (τi, τf) (assumptions_to_closed_gradual_pairs A)).
+
+Lemma 𝓕_typed (A : list Assumption) (PA : UBAssumptions A) (τi τf : cast_calculus.types.type) (P : A ⊢ τi ~ τf) :
+  (assumptions_to_context A) ⊢ₛ (𝓕 A τi τf P) : ((initial_type τi τf A) → (final_type τi τf A)).
+Proof.
+  induction P; intros.
+  - admit.
+  - admit.
+  - admit.
+  - admit.
+  - admit.
+  - admit.
+  - admit.
+  - admit.
+  - simpl. apply between_T
+    apply Lam_typed.
+    apply App_typed with (τ1 := initial_type (types.TRec τi) (types.TRec τf) A).
+    apply App_typed with (τ1 := ((initial_type (types.TRec τi) (types.TRec τf) A
+     → final_type (types.TRec τi) (types.TRec τf) A) → (initial_type (types.TRec τi) (types.TRec τf) A
+     → final_type (types.TRec τi) (types.TRec τf) A))).
+    apply Fix_typed.
+    admit. (** initial and final types are closed!! *)
+    apply Lam_typed.
+    apply Lam_typed.
+    assert (Paa : final_type (types.TRec τi) (types.TRec τf) A = TRec (final_type τi τf A)).
+    admit.
+    assert (Pbb : initial_type (types.TRec τi) (types.TRec τf) A = TRec (initial_type τi τf A)).
+    admit.
+    rewrite Paa.
+    apply Fold_typed.
+    rewrite Pbb.
+    apply App_typed with (τ1 := initial_type τi τf A).
+    apply up_type_three.
+    assert (HHH : ((final_type τi τf A) = (final_type τi τf A).[TRec (final_type τi τf A)/])).
+    admit.
+    rewrite -HHH.
+    admit.
+    admit.
+    admit.
+  - admit.
+  - admit.
+  - admit.
+  - admit.
+
+  - (** var var *)
+    simpl. apply Var_typed.
+    (** spec here!!! *)
+    admit.
+
+
+  - apply extract_typed.
+  - apply embed_typed.
+  - apply factorization_up_typed with (τG := τG); (try done || by eapply get_shape_is_ground).
+    by apply IHP.
+  - apply factorization_down_typed with (τG := τG); (try done || by eapply get_shape_is_ground).
+    by apply IHP.
+  - apply identity_typed.
+  - apply identity_typed.
+  - apply between_TSum_typed.
+    by apply IHP1.
+    by apply IHP2.
+  - apply between_TProd_typed.
+    by apply IHP1.
+    by apply IHP2.
+  - apply between_TArrow_typed.
+    by apply IHP1.
+    by apply IHP2.
+  - simpl. apply Lam_typed.
+    apply App_typed with (τ1 := TRec << τi >>).
+    apply App_typed with (τ1 := ((TRec << τi >> → TRec << τf >>) → (TRec << τi >> → TRec << τf >>))).
+    apply Fix_typed. admit.
+    apply Lam_typed. apply Lam_typed. apply Fold_typed.
+
+
+
+
+Fixpoint 𝓕 (A : list Assumption) (Σ : list nat) (τi τf : cast_calculus.types.type) (P : A ⊢ τi ~ τf) : expr :=
