theories/stlc_mu/typing.v
@@ -81,3 +81,100 @@ Proof.
 Qed.
 
 Definition Is_Closed τ := forall τ', τ.[τ'/] = τ.
+
+
+
+Lemma n_closed_invariant n (e : expr) s1 s2 :
+  (∀ f, e.[upn n f] = e) → (∀ x, x < n → s1 x = s2 x) → e.[s1] = e.[s2].
+Proof.
+  intros Hnc. specialize (Hnc (ren (+1))).
+  revert n Hnc s1 s2.
+  induction e => m Hmc s1 s2 H1; asimpl in *; try f_equal;
+    try (match goal with H : _ |- _ => eapply H end; eauto;
+         try inversion Hmc; try match goal with H : _ |- _ => by rewrite H end;
+         fail).
+  - apply H1. rewrite iter_up in Hmc. destruct lt_dec; try lia.
+    asimpl in *. injection Hmc as Hmc. unfold var in *. omega.
+  - unfold upn in *.
+    change (e.[up (upn m (ren (+1)))]) with
+    (e.[iter (S m) up (ren (+1))]) in *.
+    apply (IHe (S m)).
+    + inversion Hmc; match goal with H : _ |- _ => (by rewrite H) end.
+    + intros [|[|x]] H2; [by cbv| |].
+      asimpl; rewrite H1; auto with lia.
+      asimpl; rewrite H1; auto with lia.
+  - change (e1.[up (upn m (ren (+1)))]) with
+    (e1.[iter (S m) up (ren (+1))]) in *.
+    apply (IHe0 (S m)).
+    + inversion Hmc; match goal with H : _ |- _ => (by rewrite H) end.
+    + intros [|x] H2; [by cbv |].
+      asimpl; rewrite H1; auto with lia.
+  - change (e2.[up (upn m (ren (+1)))]) with
+    (e2.[upn (S m) (ren (+1))]) in *.
+    apply (IHe1 (S m)).
+    + inversion Hmc; match goal with H : _ |- _ => (by rewrite H) end.
+    + intros [|x] H2; [by cbv |].
+      asimpl; rewrite H1; auto with lia.
+Qed.
+
+(** Weakening *)
+Lemma context_gen_weakening ξ Γ' Γ e τ :
+  Γ' ++ Γ ⊢ₛ e : τ →
+  Γ' ++ ξ ++ Γ ⊢ₛ e.[upn (length Γ') (ren (+ (length ξ)))] : τ.
+Proof.
+  intros H1.
+  remember (Γ' ++ Γ) as Ξ. revert Γ' Γ ξ HeqΞ.
+  induction H1 => Γ1 Γ2 ξ HeqΞ; subst; asimpl in *; eauto using typed.
+  - rewrite iter_up; destruct lt_dec as [Hl | Hl].
+    + constructor. rewrite lookup_app_l; trivial. by rewrite lookup_app_l in H.
+    + asimpl. constructor. rewrite lookup_app_r; auto with lia.
+      rewrite lookup_app_r; auto with lia.
+      rewrite lookup_app_r in H; auto with lia.
+      match goal with
+        |- _ !! ?A = _ => by replace A with (x - length Γ1) by lia
+      end.
+  - econstructor; eauto. by apply (IHtyped2 (_::_)). by apply (IHtyped3 (_::_)).
+  - constructor. by apply (IHtyped (_ :: _)).
+Qed.
+
+Lemma context_weakening ξ Γ e τ :
+  Γ ⊢ₛ e : τ → ξ ++ Γ ⊢ₛ e.[(ren (+ (length ξ)))] : τ.
+Proof. eapply (context_gen_weakening _ []). Qed.
+
+Lemma closed_context_weakening ξ Γ e τ :
+  (∀ f, e.[f] = e) → Γ ⊢ₛ e : τ → ξ ++ Γ ⊢ₛ e : τ.
+Proof. intros H1 H2. erewrite <- H1. by eapply context_weakening. Qed.
+
+Lemma rename_ren (e : expr) (i : nat) : rename (+i) e = e.[ren (+i)].
+Proof.
+  by asimpl.
+Qed.
+
+Lemma up_type i Γ e τ Γ' : (length Γ' = i) -> (Γ ⊢ₛ e : τ) -> (Γ' ++ Γ) ⊢ₛ rename (+i) e : τ.
+Proof.
+  intros.
+  rewrite rename_ren.
+  simplify_eq.
+  by apply context_weakening.
+Qed.
+
+Lemma up_type_one Γ e τ τ' : (Γ ⊢ₛ e : τ) -> τ' :: Γ ⊢ₛ rename (+1) e : τ.
+Proof.
+  intro.
+  assert (T : τ' :: Γ = [τ'] ++ Γ). done. rewrite T.
+  by apply up_type.
+Qed.
+
+Lemma up_type_two Γ e τ τ' τ'' : (Γ ⊢ₛ e : τ) -> τ' :: τ'' :: Γ ⊢ₛ rename (+2) e : τ.
+Proof.
+  intros.
+  assert (T : τ' :: τ'' :: Γ = [τ' ; τ''] ++ Γ). done. rewrite T.
+  by apply up_type.
+Qed.
+
+Lemma up_type_three Γ e τ τ' τ'' τ''' : (Γ ⊢ₛ e : τ) -> τ' :: τ'' :: τ''' :: Γ ⊢ₛ rename (+3) e : τ.
+Proof.
+  intros.
+  assert (T : τ' :: τ'' :: τ''' :: Γ = [τ' ; τ'' ; τ'''] ++ Γ). done. rewrite T.
+  by apply up_type.
+Qed.
